kubernetes_model/simplereplicaset/replica_set.go
@@ -3,6 +3,7 @@ package simplereplicaset
 import (
 	"context"
 	"fmt"
+	"kubernetes_model/simpleapiserver"
 	"sort"
 	"sync"
 
@@ -10,21 +11,13 @@ import (
 	v1 "k8s.io/api/core/v1"
 	apierrors "k8s.io/apimachinery/pkg/api/errors"
 	metav1 "k8s.io/apimachinery/pkg/apis/meta/v1"
-	_ "k8s.io/apimachinery/pkg/labels"
+	"k8s.io/apimachinery/pkg/labels"
 	"k8s.io/apimachinery/pkg/runtime/schema"
 	"k8s.io/apimachinery/pkg/types"
 	utilruntime "k8s.io/apimachinery/pkg/util/runtime"
-	appslisters "k8s.io/client-go/listers/apps/v1"
-	corelisters "k8s.io/client-go/listers/core/v1"
 	"k8s.io/client-go/tools/cache"
 	"k8s.io/klog/v2"
 	"k8s.io/kubernetes/pkg/controller"
-)
-
-const (
-	// controllerUIDIndex is the name for the ReplicaSet store's index function,
-	// which is to index by ReplicaSet's controllerUID.
-	controllerUIDIndex = "controllerUID"
 )
 
 // ReplicaSetController is responsible for synchronizing ReplicaSet objects stored
@@ -35,25 +28,72 @@ type ReplicaSetController struct {
 	// For example, this struct can be used (with adapters) to handle ReplicationController.
 	schema.GroupVersionKind
 
-	podControl controller.PodControlInterface
-	// podIndexer allows looking up pods by ControllerRef UID
-	podIndexer cache.Indexer
-
 	// A ReplicaSet is temporarily suspended after creating/deleting these many replicas.
 	// It resumes normal action after observing the watch events for them.
 	burstReplicas int
-	// To allow injection of syncReplicaSet for testing.
-	syncHandler func(ctx context.Context, rsKey string) error
+}
 
-	// A TTLCache of pod creates/deletes each rc expects to see.
-	expectations *controller.UIDTrackingControllerExpectations
+func validateControllerRef(controllerRef *metav1.OwnerReference) error {
+	if controllerRef == nil {
+		return fmt.Errorf("controllerRef is nil")
+	}
+	if len(controllerRef.APIVersion) == 0 {
+		return fmt.Errorf("controllerRef has empty APIVersion")
+	}
+	if len(controllerRef.Kind) == 0 {
+		return fmt.Errorf("controllerRef has empty Kind")
+	}
+	if controllerRef.Controller == nil || !*controllerRef.Controller {
+		return fmt.Errorf("controllerRef.Controller is not set to true")
+	}
+	if controllerRef.BlockOwnerDeletion == nil || !*controllerRef.BlockOwnerDeletion {
+		return fmt.Errorf("controllerRef.BlockOwnerDeletion is not set")
+	}
+	return nil
+}
 
-	// A store of ReplicaSets, populated by the shared informer passed to NewReplicaSetController
-	rsLister  appslisters.ReplicaSetLister
-	rsIndexer cache.Indexer
+func CreatePods(ctx context.Context, namespace string, template *v1.PodTemplateSpec, controllerObject *apps.ReplicaSet, controllerRef *metav1.OwnerReference) error {
+	return CreatePodsWithGenerateName(ctx, namespace, template, controllerObject, controllerRef, "")
+}
 
-	// A store of pods, populated by the shared informer passed to NewReplicaSetController
-	podLister corelisters.PodLister
+func CreatePodsWithGenerateName(ctx context.Context, namespace string, template *v1.PodTemplateSpec, controllerObject *apps.ReplicaSet, controllerRef *metav1.OwnerReference, generateName string) error {
+	if err := validateControllerRef(controllerRef); err != nil {
+		return err
+	}
+	pod, err := controller.GetPodFromTemplate(template, controllerObject, controllerRef)
+	if err != nil {
+		return err
+	}
+	if len(generateName) > 0 {
+		pod.ObjectMeta.GenerateName = generateName
+	}
+	if len(labels.Set(pod.Labels)) == 0 {
+		return fmt.Errorf("unable to create pods, no labels")
+	}
+	_, err = simpleapiserver.PodCreate(namespace, pod)
+	return err
+}
+
+func FilterPodsByOwner(owner *metav1.ObjectMeta) ([]*v1.Pod, error) {
+	result := []*v1.Pod{}
+	// Iterate over two keys:
+	// - the UID of the owner, which identifies Pods that are controlled by the owner
+	// - the OrphanPodIndexKey, which identifies orphaned Pods in the owner's namespace and might be adopted by the owner later
+	for _, key := range []string{string(owner.UID), simpleapiserver.OrphanPodIndexKeyForNamespace(owner.Namespace)} {
+		pods, err := simpleapiserver.ByIndex("Pod", simpleapiserver.PodControllerUIDIndex, key)
+		if err != nil {
+			return nil, err
+		}
+		for _, obj := range pods {
+			pod, ok := obj.(*v1.Pod)
+			if !ok {
+				utilruntime.HandleError(fmt.Errorf("unexpected object type in pod indexer: %v", obj))
+				continue
+			}
+			result = append(result, pod)
+		}
+	}
+	return result, nil
 }
 
 func (rsc *ReplicaSetController) getReplicaSetsWithSameController(logger klog.Logger, rs *apps.ReplicaSet) []*apps.ReplicaSet {
@@ -63,7 +103,7 @@ func (rsc *ReplicaSetController) getReplicaSetsWithSameController(logger klog.Lo
 		return nil
 	}
 
-	objects, err := rsc.rsIndexer.ByIndex(controllerUIDIndex, string(controllerRef.UID))
+	objects, err := simpleapiserver.ByIndex("ReplicaSet", simpleapiserver.ControllerUIDIndex, string(controllerRef.UID))
 	if err != nil {
 		utilruntime.HandleError(err)
 		return nil
@@ -81,7 +121,7 @@ func (rsc *ReplicaSetController) getReplicaSetsWithSameController(logger klog.Lo
 // It will requeue the replica set in case of an error while creating/deleting pods.
 func (rsc *ReplicaSetController) manageReplicas(ctx context.Context, activePods []*v1.Pod, rs *apps.ReplicaSet) error {
 	diff := len(activePods) - int(*(rs.Spec.Replicas))
-	rsKey, err := controller.KeyFunc(rs)
+	_, err := controller.KeyFunc(rs)
 	if err != nil {
 		utilruntime.HandleError(fmt.Errorf("couldn't get key for %v %#v: %v", rsc.Kind, rs, err))
 		return nil
@@ -97,7 +137,6 @@ func (rsc *ReplicaSetController) manageReplicas(ctx context.Context, activePods 
 		// UID, which would require locking *across* the create, which will turn
 		// into a performance bottleneck. We should generate a UID for the pod
 		// beforehand and store it via ExpectCreations.
-		rsc.expectations.ExpectCreations(logger, rsKey, diff)
 		logger.V(2).Info("Too few replicas", "replicaSet", klog.KObj(rs), "need", *(rs.Spec.Replicas), "creating", diff)
 		// Batch the pod creates. Batch sizes start at SlowStartInitialBatchSize
 		// and double with each successful iteration in a kind of "slow start".
@@ -107,8 +146,8 @@ func (rsc *ReplicaSetController) manageReplicas(ctx context.Context, activePods 
 		// prevented from spamming the API service with the pod create requests
 		// after one of its pods fails.  Conveniently, this also prevents the
 		// event spam that those failures would generate.
-		successfulCreations, err := slowStartBatch(diff, controller.SlowStartInitialBatchSize, func() error {
-			err := rsc.podControl.CreatePods(ctx, rs.Namespace, &rs.Spec.Template, rs, metav1.NewControllerRef(rs, rsc.GroupVersionKind))
+		_, err := slowStartBatch(diff, controller.SlowStartInitialBatchSize, func() error {
+			err := CreatePods(ctx, rs.Namespace, &rs.Spec.Template, rs, metav1.NewControllerRef(rs, rsc.GroupVersionKind))
 			if err != nil {
 				if apierrors.HasStatusCause(err, v1.NamespaceTerminatingCause) {
 					// if the namespace is being terminated, we don't have to do
@@ -119,16 +158,6 @@ func (rsc *ReplicaSetController) manageReplicas(ctx context.Context, activePods 
 			return err
 		})
 
-		// Any skipped pods that we never attempted to start shouldn't be expected.
-		// The skipped pods will be retried later. The next controller resync will
-		// retry the slow start process.
-		if skippedPods := diff - successfulCreations; skippedPods > 0 {
-			logger.V(2).Info("Slow-start failure. Skipping creation of pods, decrementing expectations", "podsSkipped", skippedPods, "kind", rsc.Kind, "replicaSet", klog.KObj(rs))
-			for i := 0; i < skippedPods; i++ {
-				// Decrement the expected number of creates because the informer won't observe this pod
-				rsc.expectations.CreationObserved(logger, rsKey)
-			}
-		}
 		return err
 	} else if diff > 0 {
 		if diff > rsc.burstReplicas {
@@ -148,12 +177,8 @@ func (rsc *ReplicaSetController) manageReplicas(ctx context.Context, activePods 
 		for _, pod := range podsToDelete {
 			go func(targetPod *v1.Pod) {
 				defer wg.Done()
-				if err := rsc.podControl.DeletePod(ctx, rs.Namespace, targetPod.Name, rs); err != nil {
-					// Decrement the expected number of deletes because the informer won't observe this deletion
-					podKey := controller.PodKey(targetPod)
-					rsc.expectations.DeletionObserved(logger, rsKey, podKey)
+				if err := simpleapiserver.PodDelete(rs.Namespace, targetPod.Name); err != nil {
 					if !apierrors.IsNotFound(err) {
-						logger.V(2).Info("Failed to delete pod, decremented expectations", "pod", podKey, "kind", rsc.Kind, "replicaSet", klog.KObj(rs))
 						errCh <- err
 					}
 				}
@@ -184,7 +209,7 @@ func (rsc *ReplicaSetController) syncReplicaSet(ctx context.Context, key string)
 	if err != nil {
 		return err
 	}
-	rs, err := rsc.rsLister.ReplicaSets(namespace).Get(name)
+	rs, err := simpleapiserver.ReplicaSetGet(namespace, name)
 	if apierrors.IsNotFound(err) {
 		return nil
 	}
@@ -193,7 +218,7 @@ func (rsc *ReplicaSetController) syncReplicaSet(ctx context.Context, key string)
 	}
 
 	// List all pods indexed to RS UID and Orphan pods
-	allRSPods, err := controller.FilterPodsByOwner(rsc.podIndexer, &rs.ObjectMeta)
+	allRSPods, err := FilterPodsByOwner(&rs.ObjectMeta)
 	if err != nil {
 		return err
 	}
@@ -201,21 +226,13 @@ func (rsc *ReplicaSetController) syncReplicaSet(ctx context.Context, key string)
 	// NOTE: activePods and terminatingPods are pointing to objects from cache - if you need to
 	// modify them, you need to copy it first.
 	allActivePods := controller.FilterActivePods(logger, allRSPods)
-	// activePods, err := rsc.claimPods(ctx, rs, selector, allActivePods)
-	if err != nil {
-		return err
-	}
 
 	var manageReplicasErr error
 	if rs.DeletionTimestamp == nil {
 		manageReplicasErr = rsc.manageReplicas(ctx, allActivePods, rs)
 	}
 
-	if manageReplicasErr != nil {
-		return manageReplicasErr
-	}
-
-	return nil
+	return manageReplicasErr
 }
 
 // goose doesn't support Go's built-in min with final type int, so we define our own int
@@ -275,7 +292,7 @@ func (rsc *ReplicaSetController) getIndirectlyRelatedPods(logger klog.Logger, rs
 			// This object has an invalid selector, it does not match any pods
 			continue
 		}
-		pods, err := rsc.podLister.Pods(relatedRS.Namespace).List(selector)
+		pods, err := simpleapiserver.PodList(relatedRS.Namespace, selector)
 		if err != nil {
 			return nil, err
 		}
